user 3, session 5567, part 14

diffs-annotated-fixed/3/user-3-session-5567.v
@@ -585,13 +585,253 @@ step.
 *
 (destruct (a == a0); simplify; finish).
 Unshelve.
+{
+auto.
 }
 exact (fun _ => True).
-Add Search Blacklist "Raw" "Proofs".
-Set Search Output Name Only.
-Redirect "/var/folders/5x/1mdbpbjd7012l971fq0zkj2w0000gn/T/coqvoBkdJ"
-SearchPattern _.
-Remove Search Blacklist "Raw" "Proofs".
-Unset Search Output Name Only.
+Qed.
+Theorem fixup_stub_ok :
+  forall a,
+  proc_spec
+    (fun '(d, s) state =>
+     {|
+     pre := a < diskSize d /\
+            match s with
+            | FullySynced => True
+            | OutOfSync a' b => True
+            end;
+     post := fun r state' =>
+             match s with
+             | FullySynced => True
+             | OutOfSync a' b => True
+             end;
+     recovered := fun _ state' =>
+                  match s with
+                  | FullySynced => True
+                  | OutOfSync a' b => True
+                  end |}) (fixup a) td.recover td.abstr.
+Proof.
+Admitted.
+Hint Resolve fixup_ok: core.
+Theorem recover_at_ok :
+  forall a,
+  proc_spec
+    (fun '(d, s) state =>
+     {|
+     pre := a <= diskSize d /\
+            match s with
+            | FullySynced => disk0 state ?|= eq d /\ disk1 state ?|= eq d
+            | OutOfSync a' b =>
+                a' < a /\
+                disk0 state ?|= eq (diskUpd d a' b) /\ disk1 state ?|= eq d
+            end;
+     post := fun r state' =>
+             match s with
+             | FullySynced => disk0 state' ?|= eq d /\ disk1 state' ?|= eq d
+             | OutOfSync a' b =>
+                 disk0 state' ?|= eq d /\ disk1 state' ?|= eq d \/
+                 disk0 state' ?|= eq (diskUpd d a' b) /\
+                 disk1 state' ?|= eq (diskUpd d a' b)
+             end;
+     recovered := fun _ state' =>
+                  match s with
+                  | FullySynced =>
+                      disk0 state' ?|= eq d /\ disk1 state' ?|= eq d
+                  | OutOfSync a' b =>
+                      disk0 state' ?|= eq d /\ disk1 state' ?|= eq d \/
+                      disk0 state' ?|= eq (diskUpd d a' b) /\
+                      disk1 state' ?|= eq d \/
+                      disk0 state' ?|= eq (diskUpd d a' b) /\
+                      disk1 state' ?|= eq (diskUpd d a' b)
+                  end |}) (recover_at a) td.recover td.abstr.
+Proof.
+(induction a; simpl; intros).
+-
+step.
+(destruct s; simplify).
+-
+step.
+(destruct s; simplify).
++
+(exists d,FullySynced; simplify; finish).
+(destruct r; step).
+(exists d,FullySynced; simplify; finish).
+lia.
++
+(exists d,(OutOfSync a0 b); simplify; finish).
+intuition eauto.
+{
+lia.
+}
+{
+(destruct r; step).
+intuition.
+*
+(exists d,(OutOfSync a0 b); simplify; finish).
+lia.
+*
+(exists (diskUpd d a0 b),FullySynced; simplify; finish).
+lia.
+}
+Qed.
+Theorem recover_stub_at_ok :
+  forall a,
+  proc_spec
+    (fun (_ : unit) state =>
+     {|
+     pre := True;
+     post := fun r state' => True;
+     recovered := fun _ state' => True |}) (recover_at a) td.recover td.abstr.
+Proof.
+Admitted.
+Hint Resolve recover_at_ok: core.
+Definition Recover_spec : Specification _ unit unit TwoDiskBaseAPI.State :=
+  fun '(d, s) state =>
+  {|
+  pre := match s with
+         | FullySynced => disk0 state ?|= eq d /\ disk1 state ?|= eq d
+         | OutOfSync a b =>
+             a < diskSize d /\
+             disk0 state ?|= eq (diskUpd d a b) /\ disk1 state ?|= eq d
+         end;
+  post := fun (_ : unit) state' =>
+          match s with
+          | FullySynced => disk0 state' ?|= eq d /\ disk1 state' ?|= eq d
+          | OutOfSync a b =>
+              disk0 state' ?|= eq d /\ disk1 state' ?|= eq d \/
+              disk0 state' ?|= eq (diskUpd d a b) /\
+              disk1 state' ?|= eq (diskUpd d a b)
+          end;
+  recovered := fun (_ : unit) state' =>
+               match s with
+               | FullySynced =>
+                   disk0 state' ?|= eq d /\ disk1 state' ?|= eq d
+               | OutOfSync a b =>
+                   disk0 state' ?|= eq d /\ disk1 state' ?|= eq d \/
+                   disk0 state' ?|= eq (diskUpd d a b) /\
+                   disk1 state' ?|= eq d \/
+                   disk0 state' ?|= eq (diskUpd d a b) /\
+                   disk1 state' ?|= eq (diskUpd d a b)
+               end |}.
+Definition Recover_spec_stub :
+  Specification _ unit unit TwoDiskBaseAPI.State :=
+  fun (_ : unit) state =>
+  {|
+  pre := True;
+  post := fun _ state' => True;
+  recovered := fun _ state' => True |}.
+Theorem Recover_rok : proc_spec Recover_spec Recover td.recover td.abstr.
+Proof.
+(unfold Recover, Recover_spec; intros).
+(spec_intros; simplify).
+(destruct s; simplify).
++
+step.
+step.
+(exists d,FullySynced; simplify; finish).
+step.
++
+step.
+intuition eauto.
+{
+simplify.
+}
+step.
+(exists d,(OutOfSync a b); simplify; finish).
+step.
+Qed.
+Theorem Recover_spec_idempotent : idempotent Recover_spec.
+Proof.
+(unfold idempotent).
+(destruct a as [d st]).
+(intuition; simplify).
+(destruct st; intuition eauto).
+-
+(exists d,FullySynced; finish).
+-
+(exists d,FullySynced; finish).
+-
+(exists d,(OutOfSync a b); finish).
+-
+(exists (diskUpd d a b),FullySynced; finish).
+Qed.
+Theorem Recover_ok : proc_loopspec Recover_spec Recover td.recover td.abstr.
+Proof.
+(eapply idempotent_loopspec; simpl).
+-
+(apply Recover_rok).
+-
+(apply Recover_spec_idempotent).
+Qed.
+Hint Resolve Recover_ok: core.
+Definition recover : proc unit := _ <- td.recover; Recover.
+Definition rd_abstraction (state : TwoDiskBaseAPI.State)
+  (d : OneDiskAPI.State) : Prop :=
+  disk0 state ?|= eq d /\ disk1 state ?|= eq d.
+Definition abstr : Abstraction OneDiskAPI.State :=
+  abstraction_compose td.abstr {| abstraction := rd_abstraction |}.
+Theorem init_ok : init_abstraction init recover abstr inited_any.
+Proof.
+(intros).
+(eapply then_init_compose; eauto).
+(eapply proc_spec_weaken; eauto).
+(unfold spec_impl; intros).
+(destruct state; simpl in *).
+-
+(exists (d_0, d_1); simpl; intuition eauto).
+(unfold rd_abstraction).
+(destruct v; repeat deex; eauto).
+-
+(exists (d_0, d_0); simpl; intuition eauto).
+(unfold rd_abstraction).
+(destruct v; repeat deex; eauto).
+-
+(exists (d_1, d_1); simpl; intuition eauto).
+(unfold rd_abstraction).
+(destruct v; repeat deex; eauto).
+Qed.
+Theorem read_ok : forall a, proc_spec (read_spec a) (read a) recover abstr.
+Proof.
+(intros).
+(apply spec_abstraction_compose; simpl).
+(eapply compose_recovery; eauto; simplify).
+(unfold rd_abstraction in *; descend; intuition eauto).
+(exists (state2, FullySynced); simplify; finish).
+Qed.
+Theorem write_ok :
+  forall a v, proc_spec (write_spec a v) (write a v) recover abstr.
+Proof.
+(intros).
+(apply spec_abstraction_compose; simpl).
+(eapply compose_recovery; eauto; simplify).
+rename state2 into d.
+(unfold rd_abstraction in *; descend; intuition eauto).
+-
+(exists (d, FullySynced); simplify; intuition eauto).
+-
+(exists (d, OutOfSync a v); simplify; intuition eauto).
+-
+(exists (diskUpd d a v, FullySynced); simplify; intuition eauto).
+Qed.
+Theorem size_ok : proc_spec size_spec size recover abstr.
+Proof.
+(intros).
+(apply spec_abstraction_compose; simpl).
+(eapply compose_recovery; eauto).
+(intros; apply exists_tuple2).
+(destruct a; simpl in *).
+rename s into d.
+(unfold rd_abstraction in *; simplify).
+(exists d,d; intuition eauto).
+simplify.
+(exists d,FullySynced; simplify; finish).
+Qed.
+Theorem recover_wipe : rec_wipe recover abstr no_wipe.
+Proof.
+(eapply rec_wipe_compose; eauto; simpl).
+(autounfold; unfold rd_abstraction, Recover_spec; simplify).
+(exists state0',FullySynced; intuition eauto).
+Qed.
+End ReplicatedDisk.
 (* Auto-generated comment: Succeeded. *)
 
